Veir/Data/Refinement.lean
@@ -15,10 +15,12 @@ public section
   In particular, any concrete `i'` refines a poison `i`, but a poison `i'` does *not* refine
   any `i`.
 -/
-def isRefinedBy (i i' : Veir.Data.LLVM.Int 64) : Prop :=
+def isRefinedBy {w : Nat} (i i' : Veir.Data.LLVM.Int w) :=
   match i with
   | .val v =>
     match i' with
     | .val v' => v = v'
-    | .poison => true
+    | .poison => false
   | .poison => true
+
+@[inherit_doc] infix:50 " ⊑ "  => isRefinedBy
